Add reserved keys example

external/Goose/github_com/mit_pdos/go_mvcc/examples.v
@@ -4,10 +4,41 @@ From Goose Require github_com.mit_pdos.go_mvcc.txn.
 
 From Perennial.goose_lang Require Import ffi.grove_prelude.
 
-Definition Example1: val :=
-  rec: "Example1" "txn" :=
-    txn.Txn__Begin "txn";;
-    let: ("v0", <>) := txn.Txn__Get "txn" #0 in
-    let: ("v2", <>) := txn.Txn__Get "txn" #2 in
-    let: "total" := "v0" + "v2" in
-    "total".
+Definition WriteReservedKeySeq: val :=
+  rec: "WriteReservedKeySeq" "txn" :=
+    txn.Txn__Put "txn" #0 #2;;
+    #true.
+
+Definition WriteReservedKey: val :=
+  rec: "WriteReservedKey" "txn" :=
+    txn.Txn__DoTxn "txn" WriteReservedKeySeq.
+
+Definition WriteFreeKeySeq: val :=
+  rec: "WriteFreeKeySeq" "txn" :=
+    txn.Txn__Put "txn" #1 #3;;
+    #true.
+
+Definition WriteFreeKey: val :=
+  rec: "WriteFreeKey" "txn" :=
+    txn.Txn__DoTxn "txn" WriteFreeKeySeq.
+
+Definition WriteReservedKeyExample: val :=
+  rec: "WriteReservedKeyExample" <> :=
+    let: "mgr" := txn.MkTxnMgr #() in
+    let: "p" := ref (zero_val uint64T) in
+    txn.TxnMgr__InitializeData "mgr" "p";;
+    let: "txn" := txn.TxnMgr__New "mgr" in
+    let: "ok" := WriteReservedKey "txn" in
+    (if: "ok"
+    then "p" <-[uint64T] #2
+    else #());;
+    ("p", "ok").
+
+Definition WriteFreeKeyExample: val :=
+  rec: "WriteFreeKeyExample" <> :=
+    let: "mgr" := txn.MkTxnMgr #() in
+    let: "p" := ref (zero_val uint64T) in
+    txn.TxnMgr__InitializeData "mgr" "p";;
+    let: "txn" := txn.TxnMgr__New "mgr" in
+    let: "ok" := WriteFreeKey "txn" in
+    "ok".
