src/program_proof/mvcc/examples_proof.v
@@ -1,0 +1,335 @@
+From Perennial.program_proof Require Import grove_prelude.
+From Goose.github_com.mit_pdos.go_mvcc Require Import examples.
+From Perennial.program_proof.mvcc Require Import txn_proof.
+
+Section program.
+Context `{!heapGS Σ, !mvcc_ghostG Σ}.
+
+Definition P_WriteReservedKey (r : dbmap) := dom r = {[ (U64 0) ]}.
+Definition Q_WriteReservedKey (r w: dbmap) :=
+  w !! (U64 0) = Some (Value (U64 2)).
+
+Theorem wp_WriteReservedKeySeq txn tid r γ τ :
+  {{{ own_txn txn tid r γ τ ∗ ⌜P_WriteReservedKey r⌝ ∗ txnmap_ptstos τ r }}}
+    WriteReservedKeySeq #txn
+  {{{ w (ok : bool), RET #ok;
+      own_txn txn tid r γ τ ∗
+      if ok then ⌜Q_WriteReservedKey r w ∧ dom r = dom w⌝ ∗ txnmap_ptstos τ w else True
+  }}}.
+Proof.
+  iIntros (Φ) "(Htxn & %Hdom & Hpts) HΦ".
+  wp_call.
+
+  (***********************************************************)
+  (* txn.Put(0, 2)                                           *) 
+  (* return true                                             *) 
+  (***********************************************************)
+  assert (Helem : (U64 0) ∈ dom r) by set_solver.
+  rewrite elem_of_dom in Helem. destruct Helem as [v Hlookup].
+  wp_apply (wp_txn__Put with "[$Htxn Hpts]").
+  { iDestruct (big_sepM_lookup with "Hpts") as "Hpts"; [apply Hlookup | iFrame]. }
+  iIntros "[Htxn Hpts]".
+  wp_pures.
+  iModIntro.
+  iApply ("HΦ" $! ({[ (U64 0) := (Value (U64 2)) ]})).
+  iFrame "Htxn".
+  iSplit.
+  { iPureIntro. unfold Q_WriteReservedKey. split; [by rewrite lookup_singleton | set_solver]. }
+  unfold txnmap_ptstos.
+  rewrite big_sepM_singleton.
+  done.
+Qed.
+
+Theorem wp_WriteReservedKey (txn : loc) γ :
+  ⊢ {{{ own_txn_uninit txn γ }}}
+    <<< ∀∀ (r : dbmap), ⌜P_WriteReservedKey r⌝ ∗ dbmap_ptstos γ r >>>
+      WriteReservedKey #txn @ ↑mvccNSST
+    <<< ∃∃ (ok : bool), if ok then (∃ w, ⌜Q_WriteReservedKey r w⌝ ∗ dbmap_ptstos γ w) else dbmap_ptstos γ r >>>
+    {{{ RET #ok; own_txn_uninit txn γ }}}.
+Proof.
+  iIntros "!>".
+  iIntros (Φ) "Htxn HAU".
+  wp_call.
+
+  (***********************************************************)
+  (* return txn.DoTxn(WriteReservedKeySeq)                   *)
+  (***********************************************************)
+  wp_apply (wp_txn__DoTxn _ _ _ Q_WriteReservedKey with "[$Htxn]").
+  { unfold Q_WriteReservedKey. apply _. }
+  { unfold spec_body.
+    iIntros (tid r τ Φ') "!> HP HΦ'".
+    iApply (wp_WriteReservedKeySeq with "HP HΦ'").
+  }
+  done.
+Qed.
+
+Definition P_WriteFreeKey (r : dbmap) := dom r = {[ (U64 1) ]}.
+Definition Q_WriteFreeKey (r w: dbmap) :=
+  w !! (U64 1) = Some (Value (U64 3)).
+
+Theorem wp_WriteFreeKeySeq txn tid r γ τ :
+  {{{ own_txn txn tid r γ τ ∗ ⌜P_WriteFreeKey r⌝ ∗ txnmap_ptstos τ r }}}
+    WriteFreeKeySeq #txn
+  {{{ w (ok : bool), RET #ok;
+      own_txn txn tid r γ τ ∗
+      if ok then ⌜Q_WriteFreeKey r w ∧ dom r = dom w⌝ ∗ txnmap_ptstos τ w else True
+  }}}.
+Proof.
+  iIntros (Φ) "(Htxn & %Hdom & Hpts) HΦ".
+  wp_call.
+
+  (***********************************************************)
+  (* txn.Put(1, 3)                                           *) 
+  (* return true                                             *) 
+  (***********************************************************)
+  assert (Helem : (U64 1) ∈ dom r) by set_solver.
+  rewrite elem_of_dom in Helem. destruct Helem as [v Hlookup].
+  wp_apply (wp_txn__Put with "[$Htxn Hpts]").
+  { iDestruct (big_sepM_lookup with "Hpts") as "Hpts"; [apply Hlookup | iFrame]. }
+  iIntros "[Htxn Hpts]".
+  wp_pures.
+  iModIntro.
+  iApply ("HΦ" $! ({[ (U64 1) := (Value (U64 3)) ]})).
+  iFrame "Htxn".
+  iSplit.
+  { iPureIntro. unfold Q_WriteFreeKey. split; [by rewrite lookup_singleton | set_solver]. }
+  unfold txnmap_ptstos.
+  rewrite big_sepM_singleton.
+  done.
+Qed.
+
+Theorem wp_WriteFreeKey (txn : loc) γ :
+  ⊢ {{{ own_txn_uninit txn γ }}}
+    <<< ∀∀ (r : dbmap), ⌜P_WriteFreeKey r⌝ ∗ dbmap_ptstos γ r >>>
+      WriteFreeKey #txn @ ↑mvccNSST
+    <<< ∃∃ (ok : bool), if ok then (∃ w, ⌜Q_WriteFreeKey r w⌝ ∗ dbmap_ptstos γ w) else dbmap_ptstos γ r >>>
+    {{{ RET #ok; own_txn_uninit txn γ }}}.
+Proof.
+  iIntros "!>".
+  iIntros (Φ) "Htxn HAU".
+  wp_call.
+
+  (***********************************************************)
+  (* return txn.DoTxn(WriteFreeKeySeq)                       *)
+  (***********************************************************)
+  wp_apply (wp_txn__DoTxn _ _ _ Q_WriteFreeKey with "[$Htxn]").
+  { unfold Q_WriteFreeKey. apply _. }
+  { unfold spec_body.
+    iIntros (tid r τ Φ') "!> HP HΦ'".
+    iApply (wp_WriteFreeKeySeq with "HP HΦ'").
+  }
+  done.
+Qed.
+
+Theorem wp_WriteReservedKeyExample :
+  {{{ True }}}
+    WriteReservedKeyExample #()
+  {{{ γ (p : loc) (ok : bool), RET (#p, #ok);
+      if ok
+      then frac_ptsto γ (1 / 2)%Qp (U64 0) (Value (U64 2)) ∗ p ↦[uint64T] #(U64 2)
+      (* Still give the res above, but not set to the specified value (2). *)
+      else ∃ (v : u64), frac_ptsto γ (1 / 2)%Qp (U64 0) (Value v) ∗ p ↦[uint64T] #v
+  }}}.
+Proof.
+  iIntros (Φ) "_ HΦ".
+  wp_call.
+
+  (***********************************************************)
+  (* mgr := txn.MkTxnMgr()                                   *)
+  (* p := new(uint64)                                        *)
+  (* mgr.InitializeData(p)                                   *)
+  (* txn := mgr.New()                                        *)
+  (* ok := WriteReservedKey(txn)                             *)
+  (* if ok {                                                 *)
+  (*     *p = 2                                              *)
+  (* }                                                       *)
+  (* return p, ok                                            *)
+  (***********************************************************)
+  wp_apply wp_MkTxnMgr.
+  iIntros (γ mgr) "[Hmgr Hdbpts]".
+  wp_pures.
+  wp_apply wp_ref_of_zero; first done.
+  iIntros (p) "HpRef".
+  wp_pures.
+  wp_apply (wp_txnMgr__InitializeData with "Hmgr [$Hdbpts $HpRef]").
+  iIntros (u) "(#Hmgr & Hptsto' & HpRef)".
+  wp_pures.
+  wp_apply (wp_txnMgr__New with "Hmgr").
+  iNamed "Hmgr".
+  iIntros (txn) "Htxn".
+  wp_pures.
+  wp_apply (wp_WriteReservedKey with "Htxn").
+  iInv "Hinvdb" as "> HinvdbO" "HinvdbC".
+  iApply ncfupd_mask_intro; first set_solver.
+  iIntros "Hclose".
+  iNamed "HinvdbO".
+  iExists {[ (U64 0) := v ]}.
+  iDestruct (big_sepM_delete with "Hdbpts") as "[Hdbpt Hdbpts]".
+  { apply Hval. }
+  iSplitL "Hdbpt".
+  { unfold dbmap_ptstos. rewrite big_sepM_singleton.
+    iFrame.
+    iPureIntro. unfold P_WriteReservedKey.
+    set_solver.
+  }
+  iIntros (ok) "Hdbpt".
+  iMod "Hclose" as "_".
+  destruct ok eqn:E.
+  { (* Case COMMIT. *)
+    set v' := Value (U64 2).
+    iMod (frac_ptsto_update v' with "Hptsto Hptsto'") as "[Hptsto Hptsto']"; first apply Qp_half_half.
+    iMod ("HinvdbC" with "[- HΦ Hptsto' HpRef]") as "_".
+    { (* Close the invariant. *)
+      iNext.
+      iDestruct "Hdbpt" as (w) "[%HQ Hdbpt]".
+      unfold Q_WriteReservedKey in HQ.
+      unfold dbmap_ptstos.
+      unfold mvcc_inv_db_def.
+      set m' := <[(U64 0) := v']> m.
+      iExists m', v'.
+      iDestruct (big_sepM_lookup with "Hdbpt") as "Hdbpt".
+      { apply HQ. }
+      (* Q: Can we directly iDestruct the LHS of an iff? *)
+      iAssert (dbmap_ptstos γ m')%I with "[Hdbpt Hdbpts]" as "Hdbpts".
+      { unfold dbmap_ptstos. rewrite big_sepM_insert_delete. iFrame. }
+      iFrame.
+      iPureIntro.
+      subst m'. rewrite lookup_insert.
+      split; [done | set_solver].
+    }
+    iModIntro.
+    iIntros "Htxn".
+    wp_pures.
+    wp_store.
+    wp_pures.
+    iApply "HΦ".
+    by iFrame.
+  }
+  { (* Case ABORT. *)
+    iMod ("HinvdbC" with "[- HΦ Hptsto' HpRef]") as "_".
+    { (* Close the invariant. *)
+      iNext.
+      unfold dbmap_ptstos.
+      rewrite big_sepM_singleton.
+      unfold mvcc_inv_db_def.
+      iExists m, v.
+      iAssert (dbmap_ptstos γ m)%I with "[Hdbpt Hdbpts]" as "Hdbpts".
+      { unfold dbmap_ptstos.
+        iApply big_sepM_delete; first apply Hval.
+        iFrame.
+      }
+      iFrame.
+      iPureIntro.
+      split; [done | set_solver].
+    }
+    iModIntro.
+    iIntros "Htxn".
+    wp_pures.
+    iApply "HΦ".
+    eauto with iFrame.
+  }
+Qed.
+
+Theorem wp_WriteFreeKeyExample :
+  {{{ True }}}
+    WriteFreeKeyExample #()
+  {{{ (ok : bool), RET #ok; True }}}.
+Proof using heapGS0 mvcc_ghostG0 Σ.
+  iIntros (Φ) "_ HΦ".
+  wp_call.
+
+  (***********************************************************)
+  (* mgr := txn.MkTxnMgr()                                   *)
+  (* p := new(uint64)                                        *)
+  (* mgr.InitializeData(p)                                   *)
+  (* txn := mgr.New()                                        *)
+  (* ok := WriteFreeKey(txn)                                 *)
+  (* return ok                                               *)
+  (***********************************************************)
+  wp_apply wp_MkTxnMgr.
+  iIntros (γ mgr) "[Hmgr Hdbpts]".
+  wp_pures.
+  wp_apply wp_ref_of_zero; first done.
+  iIntros (p) "HpRef".
+  wp_pures.
+  wp_apply (wp_txnMgr__InitializeData with "Hmgr [$Hdbpts $HpRef]").
+  iIntros (u) "(#Hmgr & Hptsto' & HpRef)".
+  (* Delete the [Hptsto'] to show that [WriteFreeKey] does not require that. *)
+  iClear "Hptsto'".
+  wp_pures.
+  wp_apply (wp_txnMgr__New with "Hmgr").
+  iNamed "Hmgr".
+  iIntros (txn) "Htxn".
+  wp_pures.
+  wp_apply (wp_WriteFreeKey with "Htxn").
+  iInv "Hinvdb" as "> HinvdbO" "HinvdbC".
+  iApply ncfupd_mask_intro; first set_solver.
+  iIntros "Hclose".
+  iNamed "HinvdbO".
+  assert (Hlookup : ∃ y, m !! (U64 1) = Some y).
+  { apply elem_of_dom. set_solver. }
+  destruct Hlookup as [y Hlookup].
+  iExists {[ (U64 1) := y ]}.
+  iDestruct (big_sepM_delete with "Hdbpts") as "[Hdbpt Hdbpts]".
+  { apply Hlookup. }
+  iSplitL "Hdbpt".
+  { unfold dbmap_ptstos. rewrite big_sepM_singleton.
+    iFrame.
+    iPureIntro. unfold P_WriteFreeKey.
+    set_solver.
+  }
+  iIntros (ok) "Hdbpt".
+  iMod "Hclose" as "_".
+  destruct ok eqn:E.
+  { (* Case COMMIT. *)
+    iMod ("HinvdbC" with "[- HΦ]") as "_".
+    { (* Close the invariant. *)
+      iNext.
+      iDestruct "Hdbpt" as (w) "[%HQ Hdbpt]".
+      unfold Q_WriteFreeKey in HQ.
+      unfold dbmap_ptstos.
+      unfold mvcc_inv_db_def.
+      set v' := Value (U64 3).
+      set m' := <[(U64 1) := v']> m.
+      iExists m', v.
+      iDestruct (big_sepM_lookup with "Hdbpt") as "Hdbpt".
+      { apply HQ. }
+      (* Q: Can we directly iDestruct the LHS of an iff? *)
+      iAssert (dbmap_ptstos γ m')%I with "[Hdbpt Hdbpts]" as "Hdbpts".
+      { unfold dbmap_ptstos. rewrite big_sepM_insert_delete. iFrame. }
+      iFrame.
+      iPureIntro.
+      subst m'.
+      split; last set_solver.
+      { rewrite -Hval. by apply lookup_insert_ne. }
+    }
+    iModIntro.
+    iIntros "Htxn".
+    wp_pures.
+    by iApply "HΦ".
+  }
+  { (* Case ABORT. *)
+    iMod ("HinvdbC" with "[- HΦ]") as "_".
+    { (* Close the invariant. *)
+      iNext.
+      unfold dbmap_ptstos.
+      rewrite big_sepM_singleton.
+      unfold mvcc_inv_db_def.
+      iExists m, v.
+      iAssert (dbmap_ptstos γ m)%I with "[Hdbpt Hdbpts]" as "Hdbpts".
+      { unfold dbmap_ptstos.
+        iApply big_sepM_delete; first apply Hlookup.
+        iFrame.
+      }
+      iFrame.
+      iPureIntro.
+      split; [done | set_solver].
+    }
+    iModIntro.
+    iIntros "Htxn".
+    wp_pures.
+    by iApply "HΦ".
+  }
+Qed.
+
+End program.
