src/program_proof/mvcc/txnmgr_mk.v
@@ -9,7 +9,10 @@ Context `{!heapGS Σ, !mvcc_ghostG Σ}.
 Theorem wp_MkTxnMgr :
   {{{ True }}}
     MkTxnMgr #()
-  {{{ (γ : mvcc_names) (txnmgr : loc), RET #txnmgr; is_txnmgr txnmgr γ }}}.
+  {{{ (γ : mvcc_names) (txnmgr : loc), RET #txnmgr;
+      is_txnmgr_uninit txnmgr γ ∗
+      dbmap_ptstos γ (gset_to_gmap (Value (U64 0)) keys_all)
+  }}}.
 Proof.
   iIntros (Φ) "_ HΦ".
   wp_call.
@@ -193,8 +196,25 @@ Proof.
   replace (int.nat (U64 N_TXN_SITES)) with (length sitesL); last first.
   { unfold N_TXN_SITES in *. word. }
   rewrite firstn_all.
-  do 6 iExists _.
+  (* do 6 iExists _. *)
   (* by iFrame "# %". *)
+Admitted.
+
+
+(*****************************************************************)
+(* func (txnMgr *TxnMgr) InitializeData(p *uint64)               *)
+(*****************************************************************)
+Theorem wp_txnMgr__InitializeData (txnmgr : loc) (p : loc) (v : u64) γ :
+  is_txnmgr_uninit txnmgr γ -∗
+  {{{ dbmap_ptstos γ (gset_to_gmap (Value (U64 0)) keys_all) ∗
+      p ↦[uint64T] #v
+  }}}
+    TxnMgr__InitializeData #txnmgr #p
+  {{{ (w : u64), RET #();
+      is_txnmgr txnmgr γ ∗
+      frac_ptsto γ (1 / 2)%Qp (U64 0) (Value w) ∗
+      p ↦[uint64T] #w
+  }}}.
 Admitted.
 
 End program.
